---
output:
  pdf_document: default
  html_document: default
---
# Exercise 1.8
The exercise is to solve the following Cauchy-problem
\begin{align}
  u(x) \partial_1 u(x) + \partial_2 u(x) = 1, 
  \qquad x \in \mathbb{R}^2, 
  \ u(q,q) = 0, \ q \in \mathbb{R} 
\end{align}
with
\begin{align}
  \Sigma = \left\{ (q,q) \ | \ q \in \mathbb{R} \right\}
\end{align}
 
## Transform to normal form
The normal form is given by  
\begin{align}
  u'(x) A(x) + b(x) u(x) = f(x), \qquad x \in \Omega
  (\#eq:normal)
\end{align}
were $u'(x)$ is given by
\begin{align}
  u'(x) = \left[ \partial_1 u(x) \ \ldots \ \partial_d u(x) \right]
\end{align}
We can write our equation as
\begin{align}
  \left[ \partial_1 u(x) \ \partial_2 u(x) \right] 
  \begin{bmatrix}
    u(x) \\
    1
  \end{bmatrix}
  = 1
\end{align}
i.e. our $A(x)$ and $b(x)$ becomes
\begin{align}
  A(x) = \begin{bmatrix} u(x) \\ 1 \end{bmatrix}, \qquad
  b(x) = 1
\end{align}
which in turn gives us that \@ref(eq:normal) becomes
\begin{align}
  \nabla u(x) A(x,z) = 1
\end{align}

## Parameterizing the hypersurface
The initial hypersurface $\Sigma$ by the following
$$\gamma(q) := \begin{bmatrix} q \\ q \end{bmatrix}, \qquad q \in \mathbb{R}.$$
Taking the derivative of the parameterization yields
$$\gamma'(q) = \begin{bmatrix} 1 \\ 1 \end{bmatrix}.$$
The tangent space of $\Sigma$ becomes
$$T_{\gamma(q)}\Sigma = \left\{ \begin{bmatrix} s \\ s \end{bmatrix} \Big| \ s \in \mathbb{R}\right\}.$$
The condition that $A\Big(\gamma(q), \phi(\gamma(q))\Big) \in T_{\gamma(q)}\Sigma$ is always satisfied as $A\Big(\gamma(q), \phi(\gamma(q))\Big)$ is given by the following
$$A\Big(\gamma(q), \phi(\gamma(q))\Big) = \begin{bmatrix} 0 \\ 1\end{bmatrix}.$$
The Cauchy problem is non-characteristic in everything point contained in $\Sigma$.

## System of equations
We get the following system of equations
\begin{align}
  \partial_t x_1(t,q) &= Z(t,q) \quad&&, \ x_1(0,q) = q (\#eq:system1) \\
  \partial_t x_2(t,q) &= 1 \quad&&, \ x_2(0,q) = q (\#eq:system2) \\
  \partial_t Z(t,q) &= 1 \quad&&, \ Z(0,q) = 0 (\#eq:system3)
\end{align}
From \@ref(eq:system3) we quickly see that 
\begin{align} 
  Z(t,q) = t. (\#eq:bigz)
\end{align}
From \@ref(eq:system2) we coclude that
$$x_2(t,q) = q + t.$$
Considering \@ref(eq:system1) and \@ref(eq:bigz) we see that
\begin{align}
  x_1(t,q) &= q + \int_0^t s \ ds \\
  &= q + \frac{1}{2} t^2.
\end{align}

## Finding t and q
We will start by finding $t$, we have the following expressions
$$x_1 = q + \frac{1}{2} t^2, \qquad x_2 = q + t.$$
We can start by isolating $q$ is the second equation
$$q = x_2 - t,$$
inserting this in the first equation gives the following
\begin{align}
  x_1 &= q + \frac{1}{2} t^2 \\
  &= x_2 - t + \frac{1}{2} t^2 (\#eq:x1expression)
\end{align}
Rewriting \@ref(eq:x1expression) gives
\begin{align}
  x_1 - x_2 + \frac{1}{2} = \frac{1}{2}\underbrace{\left(t^2 - 2t + 1\right)}_{(t - 1)^2}(\#eq:texpression)
\end{align}
Multiplying both sides of \@ref(eq:texpression) by $2$ gives
\begin{align}
  (t - 1)^2 &= 2x_1 - 2x_2 + 1 \\
  t - 1 &= \pm\sqrt{2x_1 - 2x_2 + 1} \\
  t &= 1 \pm\sqrt{2x_1 - 2x_2 + 1} (\#eq:psi1)
\end{align}
