---
output:
  html_document: default
  pdf_document: default
---

# Exam Exercises

## Mock exam 1

### Exercise 1
Let 
$$\Omega:=(0,\infty)^2.$$
Calculate the solution to the following Cauchy-Problem,
\begin{align*}
  &x_1\partial_1u(x) + x_2\partial_2u(x) + x_1x_2u(x) = 0, \quad x \in \Omega; \\
  &u(q,q^2) = 5, \quad q > 0.
\end{align*}

\textbf{Solution}
As the exercise does not ask if the problem is non-characteristic, we suppose that it is.
The first step is to bring the problem to normal form.
The normal form is given by 
$$\nabla u(x)A(x) + u(x)b(x) = f(x).$$
In our case 
$$A(x) = \begin{bmatrix} x_1 \\ x_2 \end{bmatrix}, \quad b(x) = x_1x_2 \quad \text{and} \quad f(x) = 0.$$

Next we want to parameterize the hypersurface, which becomes $$\gamma(q) := \begin{bmatrix} q \\ q^2 \end{bmatrix}.$$
When then seek 
$$\Phi(t,x),$$ 
which we find as the solution to 
$$\partial\Phi(t,x) = A(\Phi(t,x)).$$
As we in our case have $d = 2$ the ODE can be written as the following system
\begin{align*}
  \varphi_1'(t) &= A(\Phi(t))_1, \quad \varphi_1(0) = x_1 \\
  \varphi_2'(t) &= A(\Phi(t))_2, \quad \varphi_2(0) = x_2,
\end{align*}
by the definiton of $A(x)$ the system becomes
\begin{align*}
  \varphi_1'(t) &= \varphi(t)_1, \quad \varphi_1(0) = x_1 \\
  \varphi_2'(t) &= \varphi(t)_2, \quad \varphi_2(0) = x_2.
\end{align*}
By solving the system we get the following $\Phi(t,x)$ 
$$\Phi(t,x) = \begin{bmatrix} \varphi_1(t,x) \\ \varphi_2(t,x) \end{bmatrix} = \begin{bmatrix} x_1e^t \\ x_2e^t \end{bmatrix}.$$
By Lemma 1.8 we have $X(t,q) = \Phi(t, \gamma(q))$, thus $$X(t,q) = \Phi(t,\gamma(q)) =  \begin{bmatrix} qe^t \\ q^2e^t \end{bmatrix}.$$
As we seek values for $t$ and $q$ we can now invert the functions
\begin{align*}
  x_1 &= qe^t \\
  x_2 &= q^2e^t
\end{align*}
Isolating $q$ in the first equation gives 
$$x_1 = qe^t \Leftrightarrow e^{-t}x_1 = q,$$
Inserting this in the second equation yields
$$x_2 = \left(e^{-t}x_1\right)^2e^t 
= e^{-2t}x_1^2e^t
= e^{-t}x_1^2 
= \frac{1}{e^{t}} x_1^2,$$
this in turn gives
$$x_2 = \frac{1}{e^{t}} x_1^2
\quad \Leftrightarrow \quad
e^t = \frac{x_1^2}{x_2}\\
\quad \Leftrightarrow \quad
\log\left(e^t\right) = \log\left(\frac{x_1^2}{x_2}\right)
\quad \Leftrightarrow \quad
t = \log\left(x_1^2\right) - \log\left(x_2\right).$$
The expression we have now found for $t$ can be inserted into the expression for $x_1$ to get $q$
$$q = x_1 e^{-\left(\log\left(x_1^2\right) - \log\left(x_2\right)\right)}
= x_1 e^{\log\left(x_2\right)-\log\left(x_1^2\right)}
= x_1 \frac{x_2}{x_1^2} = \frac{x_2}{x_1}.$$
To sum up we have now found both $t$ and $q$ as
$$t = \log\left(x_1^2\right) - \log\left(x_2\right), \quad q = \frac{x_2}{x_1}.$$
We can now insert in Theorem 1.9 what we have found.
The theorem states that
$$Z(t,q) = \phi(\gamma(q))e^{-\int_0^tb(X(s,q))ds} + \int_0^t e^{-\int_s^tb(X(r,q))dr}f(X(s,q))ds,$$
with $\phi(\gamma(q))$ being $Z(0,q)$ i.e. the given initial value.
Inserting what we now, especially that $f(x) = 0$, yields
$$Z(\log\left(x_1^2\right) - \log\left(x_2\right),\frac{x_2}{x_1}) = 5 e^{-q^3\int_0^{\log\left(x_1^2\right) - \log\left(x_2\right)} e^{2s}ds} \\
= 5 e^{-q^3 \left[\frac{1}{2}e^{2s}\right]_0^{\log\left(x_1^2\right) - \log\left(x_2\right)}} \\
= 5 e^{-q^3 \frac{1}{2} 
\left(e^{2\left(\log\left(x_1^2\right) - \log\left(x_2\right)\right)} - e^0\right)} \\
= 5 e^{-q^3 \frac{1}{2} \left( e^{2\log\left(\frac{x_1^2}{x_2}\right)} - e^0\right)} \\
= 5 e^{-q^3 \frac{1}{2} \left( e^{\log\left(\frac{x_1^4}{x_2^2}\right)} - e^0\right)} \\
= 5 e^{-q^3 \frac{1}{2} \left( \frac{x_1^4}{x_2^2} - 1\right)} \\
= 5 e^{-\frac{x_2^3}{x_1^3} \frac{1}{2} \left( \frac{x_1^4}{x_2^2} - 1\right)} \\
= 5 e^{-\frac{1}{2} \left( \frac{x_1^4x_2^3}{x_1^3x_2^2} - \frac{x_2^3}{x_1^3}\right)} \\
= 5 e^{-\left(x_1x_2 - x_2^3/x_1^3\right)/2}.$$
Which in turns implies that
$$u(x) = 5 e^{-\left(x_1x_2 - x_2^3/x_1^3\right)/2}, \quad x \in \Omega.$$

### Exercise 2
Let
$$\Omega := \left\{ x \in \mathbb{R}^2 \ \Bigg| \ \ |x_1 - x_2| < \frac{\pi}{2} \right\}$$
Calculate the solution for the Cauchy problem given by
$$\frac{2}{1 + u(x)^2}\partial_1 u(x) + \frac{1}{1 + u(x)^2}\partial_2 u(x) = 1, \quad x \in \Omega \\
u(q,q) = 0, \quad q \in \mathbb{R}.$$

**Solution**
We start by rewriting to normal form
\begin{align*}
  \frac{2}{1 + u(x)^2}\partial_1 u(x) + \frac{1}{1 + u(x)^2}\partial_2 u(x) &= 1 \\
  u'(x)A(x,u(x)) &= b(x,u(x))
\end{align*}
for
\begin{align*}
  u'(x) = \left[ \partial_1 u(x) \ \partial_2 u(x) \right], \quad
  A(x,u(x)) = \begin{bmatrix} \dfrac{2}{1 + u(x)^2} \\ \dfrac{1}{1 + u(x)^2} \end{bmatrix}, \quad
  b(x,u(x)) = 1.
\end{align*}
From Lemma 1.15 we need to solve the following system, notice that the initial condition originate from $u(q,q) = 0$.
\begin{align*}
  \partial_t X_1(t,q) &= A(X(t,q), Z(t,q))_1, \quad &&X_1(0,q) = q \\
  \partial_t X_2(t,q) &= A(X(t,q), Z(t,q))_2, \quad &&X_2(0,q) = q \\
  \partial_t Z(t,q) &= b(X(t,q), Z(t,q)), \quad &&Z(0,q) = 0.
\end{align*}
Inserting what we have found so far yields the following system
\begin{align*}
  \partial_t X_1(t,q) &= \dfrac{2}{1 + Z(t,q)^2}, \quad &&X_1(0,q) = q \\
  \partial_t X_2(t,q) &= \dfrac{1}{1 + Z(t,q)^2}, \quad &&X_2(0,q) = q \\
  \partial_t Z(t,q) &= 1, \quad &&Z(0,q) = 0.
\end{align*}
As $Z(t,q)$ is present in the first to equation, we will start by solving this, then we will insert this in the other two equations and then solve these
\begin{align*}
  Z(t,q) &= t \\
  X_1(t,q) &= 2\tan^{-1}(t) + q \\
  X_2(t,q) &= \tan^{-1}(t) + q.
\end{align*}
We now need to isolate $t$ and $q$ in the to last equations, i.e. 2 equations with 2 unknowns.
$$x_2 = \tan^{-1}(t) + q 
\ \Leftrightarrow \ 
x_2 - q = \tan^{-1}(1)
\ \Leftrightarrow \
\tan(x_2 - q) = t.$$
$$x_1 = 2\tan^{-1}(t) + q
\ \Leftrightarrow \
x_1 = 2(x_2 - q) + q
\ \Leftrightarrow \
x_1 = 2x_2 - q
\ \Leftrightarrow \
q = 2x_2 - x_1.$$
$$t = \tan(x_2 - q) = \tan(x_2 - (2x_2 - x_1)) = \tan(x_1 - x_2).$$
As suggested by Theorem 1.16 we have
$$u(x) = Z(\Psi(x)) = \tan(x_1 - x_2).$$

### Exercise 3
Solve the following initial-value-problem
$$(\partial_t^2 - \partial_x^2)u(t,x) = 0, \quad t,x \in \mathbb{R} \\
u(0,x) = \cos(x), \quad \partial_tu(0,x) = \cos^3(x), \quad x \in \mathbb{R}.$$
*Hint*: $\cos^3(y) = \cos(y) - \sin^2(y)\cos(y)$

**Solution**:
Because we have $d=1$ we can use d'Alemberts formula, recognizing that problem is in fact a wave equation.

Remember that $u(0,x) = g(x)$ and that $\partial_tu(0,x) = h(x)$, i.e.
$$g(x) = \cos(x), \quad h(x) = \cos^3(x).$$
D'Alamberts formula is given by
$$u(t,x) = \frac{1}{2}\left\{g(x + t) - g(x - t)\right\} + \frac{1}{2}\int_{x-t}^{x+t}h(y)\text{d}y.$$
We insert what we know and calculate
$$u(t,x) = \frac{1}{2}\left\{\cos(x + t) - \cos(x - t)\right\} + \frac{1}{2}\int_{x-t}^{x+t}\cos^3(y)\text{d}y \\
= \frac{1}{2}\left\{\cos(x + t) - \cos(x - t)\right\} + \frac{1}{2}\int_{x-t}^{x+t}\cos(y) - \sin^2(y)\cos(y)\text{d}y \\
= \frac{1}{2}\left\{\cos(x + t) - \cos(x - t)\right\} + \frac{1}{2}\int_{x-t}^{x+t}\cos(y)\text{d}y - \frac{1}{2}\int_{x-t}^{x+t}\sin^2(y)\cos(y)\text{d}y \\
= \frac{1}{2}\left\{\cos(x + t) - \cos(x - t)\right\} + \frac{1}{2}[\sin(y)]_{x-t}^{x+t} - \frac{1}{2}\int_{x-t}^{x+t}\sin^2(y)\cos(y)\text{d}y \\
= \frac{1}{2}\left\{\cos(x + t) - \cos(x - t) + \sin(x + t) - \sin(x - t)\right\} - \frac{1}{2}\int_{x-t}^{x+t}\sin^2(y)\cos(y)\text{d}y,$$
what remains is to calculate the last antiderivative, which we will do below using substitution
$$u = \sin(x), \quad \frac{\text{d}u}{\text{d}y} = \cos(y) \ \Leftrightarrow \ \text{d}u = \cos(y)\text{d}y.$$
We can now insert this into the antiderivative remembering that we also need to substitute the bounds, i.e. applying the function $u$ on them
$$\frac{1}{2}\int_{x-t}^{x+t}\sin^2(y)\cos(y)\text{d}y \ \Leftrightarrow \ \frac{1}{2}\int_{x-t}^{x+t}\sin^2(y)\cos(y)\text{d}y \\
\Leftrightarrow \ \frac{1}{2}\int_{\sin(x-t)}^{\sin(x+t)}u^2\text{d}u \ \Leftrightarrow \ \frac{1}{6}[u^3]_{\sin(x-t)}^{\sin(x+t)} \ \Leftrightarrow \ \frac{1}{6}\left(\sin^3(x + t) - \sin^3(x - t)\right).$$
Inserting what we just found, we have expressed the solution explicitly as
$$u(t,x) = \frac{1}{2}\left\{\cos(x + t) - \cos(x - t) + \sin(x + t) - \sin(x - t)\right\} - \frac{1}{6}\left(\sin^3(x + t) - \sin^3(x - t)\right).$$